wftype.v
@@ -1,0 +1,97 @@
+From mathcomp Require Import ssreflect ssrfun ssrbool ssrnat seq fintype.
+From mathcomp Require Import eqtype fingraph path order choice. 
+From event_struct Require Import utilities.
+Require Import Equations.Prop.Loader.
+
+Set Implicit Arguments.
+Unset Strict Implicit.
+Unset Printing Implicit Defensive.
+
+Import Order.LTheory.
+Open Scope order_scope.
+
+Notation ordType := (orderType tt).
+
+Section WfDef.
+
+Context {T : Type} (r : rel T).
+
+Inductive acc_bool (x : T) :=
+  acc_bool_intro of (forall y : T, r y x -> acc_bool y).
+
+Definition well_founded_bool := forall x, acc_bool x.
+
+End WfDef.
+
+Module WellFounded.
+
+Section ClassDef.
+
+Definition mixin_of T0 (b : Order.POrder.class_of T0) (T := Order.POrder.Pack tt b) :=
+  well_founded_bool (<%O : rel T).
+
+Set Primitive Projections.
+
+Record class_of (T : Type) := Class {
+  base   : Order.POrder.class_of T;
+  mixin  : mixin_of base;
+}.
+
+Unset Primitive Projections.
+
+Local Coercion base : class_of >-> Order.POrder.class_of.
+
+Structure type (disp : unit) := Pack { sort; _ : class_of sort }.
+
+Local Coercion sort : type >-> Sortclass.
+
+Variables (T : Type) (disp : unit) (cT : type disp).
+
+Definition class := let: Pack _ c as cT' := cT return class_of cT' in c.
+
+Definition eqType := @Equality.Pack cT class.
+Definition choiceType := @Choice.Pack cT class.
+Definition porderType := @Order.POrder.Pack disp cT class.
+End ClassDef.
+
+Module Exports.
+
+Notation wfType := (type tt).
+Coercion base : class_of >-> Order.POrder.class_of.
+Coercion mixin : class_of >-> mixin_of.
+Coercion sort : type >-> Sortclass.
+Coercion eqType : type >-> Equality.type.
+Coercion choiceType : type >-> Choice.type.
+Coercion porderType : type >-> Order.POrder.type.
+Canonical eqType.
+Canonical choiceType.
+Canonical porderType.
+
+End Exports.
+
+End WellFounded.
+
+Export WellFounded.Exports.
+
+Section WfInduction.
+
+Context {T : wfType}.
+
+Lemma wf : well_founded_bool (<%O : rel T).
+Proof. by case: T=> ? []. Qed.
+
+Lemma wf_ind (P : T -> Type) :
+  (forall n, (forall m, m < n -> P m) -> P n) ->
+  forall n, P n.
+Proof.
+  move=> accP M.
+  by elim: (wf M) => ?? /accP. 
+Qed.
+
+Global Instance wf_wfType : 
+  Equations.Prop.Classes.WellFounded (<%O : rel T).
+Proof.
+  apply: wf_ind. by constructor.
+Qed.
+
+End  WfInduction.
